Correctness proof for ping protocol (#29)
* Inital simplification refactoring of keys, encryptions, signatures.

* Find keys and add to heap upon receiving message, or decrypting message

* Spike of simulation relation statement

* adding labels to ideal world

* Start Ping Protocol simulation relation.  Wait for now to get IdealWorld update

* issue-less change since it's so fundamental to the real world model

* Simple ping proof stuck

* Remove some cruft

* Some proof automation.  The simulation relation is clearly not right yet.  Not sure this is the right approach

* Successful proof of ping simulation

* Some more automation

* Automated simulation proof.  Working on top level proof.

* WIP.  Need to get a transitivity-like theorem implemented

* Fiddling with some proof automation setup.

* WIP

* Top level proof done.

* Starting to automate proof

* Some proof automation

* neatening up

* Refactoring semantics of simulates.  WIP

* Refactoring WIP

* Finished (needs more automation) proof of ping simulation relation

* Ping protocol proof done again.

* Ping Protocol Correct

* Ping protocol automation

* Remove Makefile.coq.conf which shouldn't be checked in

* More proof automation in Simulates

KeyManagement/IdealWorld.v
@@ -1,9 +1,9 @@
 From Coq Require Import String.
 From Coq Require Import Bool.Sumbool.
 Require Import Frap.
-Set Implicit Arguments.
 
-Definition user_id := var.
+Require Import Common.
+Set Implicit Arguments.
 
 Definition channel_id := nat.
 
@@ -24,6 +24,7 @@ Inductive message : Type -> Type :=
 Inductive exmsg : Type :=
 | Exm {A : Type} (msg : message A) : exmsg.
 
+(* shouldn't this be just Permissions ? *)
 Definition channels := fmap channel_id (set exmsg).
 
 Inductive cmd : Type -> Type :=
@@ -33,15 +34,27 @@ Inductive cmd : Type -> Type :=
 | Recv {msg_ty : Type} (ch_id : channel_id) : cmd (message msg_ty)
 | CreateChannel : cmd channel_id.
 
-Notation "x <- c1 ; c2" := (Bind c1 (fun x => c2)) (right associativity, at level 75).
+Module IdealNotations.
+  Notation "x <- c1 ; c2" := (Bind c1 (fun x => c2)) (right associativity, at level 75) : idealworld_scope.
+  Delimit Scope idealworld_scope with idealworld.
+End IdealNotations.
 
-Record user :=
-  { protocol : cmd unit ;
+Import IdealNotations.
+Open Scope idealworld_scope.
+
+Record user A :=
+  { protocol : cmd A ;
     perms : permissions }.
 
-Record universe := construct_universe
-                     { channel_vector : fmap channel_id channels ;
-                       users : fmap user_id user}.
+Record universe A :=
+  construct_universe {
+      channel_vector : channels (* fmap channel_id channels *)
+    ; users : user_list (user A)
+    }.
+
+(* Record universe := construct_universe *)
+(*                      { channel_vector : channels ; *)
+(*                        users : fmap user_id user}. *)
 
 (* write as inductive relation *)
 Fixpoint chs_search {A} (m : message A) : list (channel_id * permission) :=
@@ -51,12 +64,13 @@ Fixpoint chs_search {A} (m : message A) : list (channel_id * permission) :=
   | MsgPair m1 m2 => chs_search m1 ++ chs_search m2        
   end.
 
-Definition permission_subset p1 p2 : Prop :=
-  p1 = construct_permission true true \/
-  (p1 = construct_permission true false /\ p2.(write) = false) \/
-  (p1 = construct_permission false true /\ p2.(read) = false) \/
-  (p1 = construct_permission false false /\
-   p2 = construct_permission false false).
+Inductive permission_subset : permission -> permission -> Prop :=
+| ReadWriteCase : forall p2,
+    permission_subset (construct_permission true true) p2
+| WriteCase : forall b,
+    permission_subset (construct_permission false true) (construct_permission false b)
+| ReadCase : forall b,
+    permission_subset (construct_permission true false) (construct_permission b false).
 
 Fixpoint msg_permissions_valid {A} (m : message A) ps : Prop :=
   List.Forall
@@ -78,7 +92,7 @@ Inductive step_user : forall A, channels * cmd A * permissions -> channels * cmd
 | StepBindRecur : forall result result' (c1 c1' : cmd result') (c2 : result' -> cmd result) cv cv' ps ps',
     step_user (cv, c1, ps) (cv', c1', ps') ->
     step_user (cv, (Bind c1 c2), ps) (cv', (Bind c1' c2), ps')
-| StepBindProceed : forall (result result' : Set) (v : result') (c2 : result' -> cmd result) cv ps,
+| StepBindProceed : forall (result result' : Type) (v : result') (c2 : result' -> cmd result) cv ps,
     step_user (cv, (Bind (Return v) c2), ps) (cv, c2 v, ps)
 | StepCreateChannel : forall ch_id cv ps,
     ~(ch_id \in dom cv) ->
@@ -88,10 +102,59 @@ Inductive step_user : forall A, channels * cmd A * permissions -> channels * cmd
     ps $? ch_id = Some {| read := b ; write := true |} ->
     cv $? ch_id = Some ch_d ->
     msg_permissions_valid m ps ->
-    step_user (cv, Send m ch_id, ps) (cv $+ (ch_id, {Exm m} \cup ch_d) , Return tt, ps)
-| StepRecv : forall A (cv cv' : channels) ch_d ps (m : message A) ch_id (ms ms' : list (user_id * exmsg)) b,
+    step_user (cv, Send m ch_id, ps) (cv $+ (ch_id, {Exm m} \cup ch_d), Return tt, ps)
+| StepRecv : forall A (cv : channels) ch_d ps (m : message A) ch_id b,
     cv $? ch_id = Some ch_d ->
     ps $? ch_id = Some {| read := true ; write := b |} ->
     (Exm m) \in ch_d ->
     step_user (cv, Recv ch_id, ps)
               (cv, Return m, add_chs_to_set (chs_search m) ps).
+
+
+Lemma StepSend' : forall A cv cv' (m : message A) ch_id ps ch_d b,
+    ps $? ch_id = Some {| read := b ; write := true |}
+    -> cv $? ch_id = Some ch_d
+    -> msg_permissions_valid m ps
+    -> cv' = cv $+ (ch_id, {Exm m} \cup ch_d)
+    -> step_user (cv, Send m ch_id, ps) (cv', Return tt, ps).
+Proof.
+  intros; subst; econstructor; eauto.
+Qed.
+
+Lemma StepRecv' : forall A (cv : channels) ch_d ps ps' (m : message A) ch_id b,
+    cv $? ch_id = Some ch_d
+    -> ps $? ch_id = Some {| read := true ; write := b |}
+    -> (Exm m) \in ch_d
+    -> ps' = add_chs_to_set (chs_search m) ps
+    -> step_user (cv, Recv ch_id, ps)
+                (cv, Return m, ps').
+Proof.
+  intros; subst; econstructor; eauto.
+Qed.
+
+Inductive step_universe : forall {A : Type}, universe A -> universe A -> Prop :=
+| StepUser : forall A (U : universe A) u_id u proto chans perms',
+    In (u_id,u) U.(users)
+    -> step_user (U.(channel_vector), u.(protocol), u.(perms)) (chans, proto, perms')
+    -> step_universe U (construct_universe
+                         chans
+                         (updateUserList U.(users) u_id {| protocol := proto ; perms := perms' |})).
+
+
+Lemma StepUser' : forall A (U U': universe A) u_id u proto chans perms',
+    In (u_id,u) U.(users)
+    -> step_user (U.(channel_vector), u.(protocol), u.(perms)) (chans, proto, perms')
+    -> U' = (construct_universe
+              chans
+              (updateUserList U.(users) u_id {| protocol := proto ; perms := perms' |}))
+    -> step_universe U U'.
+Proof.
+  intros. subst. econstructor; eauto.
+Qed.
+
+
+Definition extractContent {A} (msg : message A) : option A :=
+  match msg with
+  | Content t => Some t
+  | _         => None
+  end.
