KeyManagement/Simulation.v
@@ -1,28 +1,29 @@
-(* From Coq Require Import Basics. *)
-Require Import Frap.
+From Coq Require Import List Classical ClassicalEpsilon.
+Require Import Frap Eqdep.
 
-Require Import Common.
+Require Import Common. 
 Require IdealWorld.
 Require RealWorld.
 
+Import IdealWorld.IdealNotations.
+Import RealWorld.RealWorldNotations.
+
 Set Implicit Arguments.
 
-
-
 Definition idealWorldIsReallyFinalState {A} (U : IdealWorld.universe A) : Prop :=
-  Forall (fun '(_,prog) => exists a, prog = IdealWorld.Return a) U.(IdealWorld.users).
+  Forall (fun '(_,u_data) => exists a, u_data.(IdealWorld.protocol) = IdealWorld.Return a) U.(IdealWorld.users).
 
 Definition realWorldIsReallyFinalState {A} (U : RealWorld.universe A) : Prop :=
   Forall (fun '(_,u_data) => exists a, u_data.(RealWorld.protocol) = RealWorld.Return a) U.(RealWorld.users).
 
-Definition idealWorldReturnOf {A} (c : IdealWorld.cmd A) : option A :=
-  match c with
+Definition idealWorldReturnOf {A} (c : IdealWorld.user A) : option A :=
+  match c.(IdealWorld.protocol) with
   | IdealWorld.Return a => Some a
   | _                   => None
   end.
 
 Definition realWorldReturnOf {A} (c : RealWorld.user_data A) : option A :=
-  match c.(RealWorld.protocol) with
+  match c.(RealWorld.protocol) with 
   | RealWorld.Return a => Some a
   | _                  => None
   end.
@@ -37,78 +38,189 @@ Fixpoint returnsOfHelper {B : Type} {A : Type -> Type} (users : user_list (A B))
     end
   end.
 
-(* Fixpoint idealWorldReturnsOf' {A} (users : user_list (IdealWorld.cmd A)) : list A := *)
-(*   match users with *)
-(*   | []      => [] *)
-(*   | (_,c) :: xs => *)
-(*     match idealWorldReturnOf c with *)
-(*     | Some a => a :: idealWorldReturnsOf' xs *)
-(*     | None   => idealWorldReturnsOf' xs *)
-(*     end *)
-(*     (* match c in (IdealWorld.cmd A') return (list A' -> list A') with *) *)
-(*     (* | IdealWorld.Return a => fun xs => a :: xs *) *)
-(*     (* | _                   => fun xs => xs *) *)
-(*     (* end (idealWorldReturnsOf' xs) *) *)
-(*   end. *)
-
 Definition idealWorldReturnsOf {A : Type} (U : IdealWorld.universe A) : list A :=
   returnsOfHelper U.(IdealWorld.users) idealWorldReturnOf.
 
 Definition realWorldReturnsOf {A : Type} (U : RealWorld.universe A) : list A :=
   returnsOfHelper U.(RealWorld.users) realWorldReturnOf.
 
+Definition finalAnswerInclusion {A} (U1 : RealWorld.universe A) (U2 : IdealWorld.universe A) :=
 
+  forall finalStateOfU1, RealWorld.step_universe^* U1 finalStateOfU1
+                    -> realWorldIsReallyFinalState finalStateOfU1
+                    -> exists finalStateOfU2, IdealWorld.step_universe^* U2 finalStateOfU2
+                                        /\ idealWorldIsReallyFinalState finalStateOfU2
+                                        /\ realWorldReturnsOf finalStateOfU1 = idealWorldReturnsOf finalStateOfU2.
 
-Definition finalAnswerInclusion {A} (U1 : IdealWorld.universe A) (U2 : RealWorld.universe A) :=
+Definition simulates {A : Type} (R : RealWorld.universe A -> IdealWorld.universe A -> Prop)
+           (U1 : RealWorld.universe A) (U2 : IdealWorld.universe A) :=
+  (forall U1 U2,
+      R U1 U2
+      -> forall U1',
+        RealWorld.step_universe U1 U1'
+        -> exists U2',
+          IdealWorld.step_universe^* U2 U2'
+          /\ R U1' U2')
 
-  forall finalStateOfU1, IdealWorld.step_universe^* U1 finalStateOfU1
-                    -> idealWorldIsReallyFinalState finalStateOfU1
-                    -> exists finalStateOfU2, RealWorld.step_universe^* U2 finalStateOfU2
-                                        /\ realWorldIsReallyFinalState finalStateOfU2
-                                        /\ idealWorldReturnsOf finalStateOfU1 = realWorldReturnsOf finalStateOfU2.
+  /\ (forall U1 U2,
+        R U1 U2
+        -> realWorldIsReallyFinalState U1
+        -> idealWorldIsReallyFinalState U2
+          /\ realWorldReturnsOf U1 = idealWorldReturnsOf U2)
 
+  /\ R U1 U2.
 
-
-
-
-
-
-(* multi step relation for some users in U1 *)
-
-
-
-
-Definition stepSilent (U1 U2 : u)   := step_universe U1 Silent U2.
-Definition kstepSilent (U1 U2 : ku) := Keys.step_universe U1 Keys.Silent U2.
-
-Inductive actionCorrespondance : observable -> Keys.Observable -> Prop :=
-| EqSendPlain : forall {A : Set} o ko usr1 usr2 (msg1 : A) (msg2 : Keys.message A),
-    o = Output usr1 msg1
-    -> ko = Keys.Output usr2 msg2
-    (* Something here about equality of messages and users.
-     * Will eventually need to handle the notion of encryption! *)
-    -> msg2 = Keys.Plaintext msg1 (* sending the same body!! *)
-    -> actionCorrespondance o ko.
- 
-Definition simulates (R : u -> ku -> Prop) (U : u) (KU : ku) :=
-  (forall U KU, R U KU
-           -> forall U', stepSilent U U'
-                   -> exists KU', kstepSilent^* KU KU'
-                            /\ R U' KU')
-
-  /\ (forall U KU, R U KU
-             -> forall a1 a2 U', step_universe U (Visible a1) U'
-                       -> exists KU' KU'', kstepSilent^* KU KU'
-                                     /\ Keys.step_universe KU' (Keys.Visible a2) KU''
-                                     (* We may eventually need here to handle multiple
-                                      * real world steps in order to collect the things
-                                      * needed to ensure the same cryptographic properties
-                                      * hold between the two universes *)
-                                     /\ actionCorrespondance a1 a2
-                                     /\ R U' KU'')
-  
-
-  /\ R U KU.
-
-Definition refines (U1 : u) (U2 : ku) :=
+Definition refines {A : Type} (U1 : RealWorld.universe A)(U2 : IdealWorld.universe A) :=
   exists R, simulates R U1 U2.
+
+Infix "<|" := refines (no associativity, at level 70).
+
+Hint Constructors IdealWorld.step_user IdealWorld.step_universe trc.
+Hint Resolve in_eq in_cons.
+
+Ltac invert H :=
+  (FrapWithoutSets.invert H || (inversion H; clear H));
+  repeat match goal with
+         (* | [ x : _ |- _ ] => subst x *)
+         | [ H : existT _ _ _ = existT _ _ _ |- _ ] => apply inj_pair2 in H; try subst
+         end.
+  
+Lemma addKeyTwice :
+  forall K V (k : K) (v v' : V) m,
+    m $+ (k, v) $+ (k, v') = m $+ (k, v').
+Proof.
+  intros. maps_equal.
+Qed.
+
+(* Question for Adam.  Is there a better way to do this??? *)
+Section decide.
+  Variable P : Prop.
+
+  Lemma decided : inhabited (sum P (~P)).
+  Proof.
+    destruct (classic P).
+    constructor; exact (inl _ H).
+    constructor; exact (inr _ H).
+  Qed.
+
+  Definition decide : sum P (~P) :=
+    epsilon decided (fun _ => True).
+End decide.
+
+Lemma addRemoveKey : 
+  forall K V (k : K) (v : V) m,
+    m $? k = None
+    -> m $+ (k,v) $- k = m.
+Proof.
+  intros.
+  eapply fmap_ext.
+  intros.
+
+  destruct (decide (k0 = k)).
+  * subst. simplify. eauto.
+  * symmetry.
+    rewrite <- lookup_add_ne with (k := k) (v := v); auto.
+    rewrite lookup_remove_ne; auto.
+Qed.
+
+Theorem lookup_empty_not_Some :
+  forall K V (k : K) (v : V),
+    empty K V $? k = Some v -> False.
+Proof.
+  intros.
+  apply lookup_Some_dom in H.
+  rewrite dom_empty in H. invert H.
+Qed.
+
+Hint Rewrite addKeyTwice addRemoveKey.
+Hint Resolve lookup_add_eq lookup_empty lookup_empty_not_Some.
+Hint Resolve IdealWorld.StepUser' IdealWorld.StepSend' IdealWorld.StepRecv'.
+
+Ltac fixcontext :=
+  match goal with
+  | [ H : $0 $? _ = Some _ |- _ ] => apply lookup_empty_not_Some in H; contradiction
+  | [ H : (_ $+ (_, _)) $? _ = Some _ |- _ ] => apply lookup_split in H; propositional; subst
+  | [ H : (_, _) = (_,_) |- _ ] => invert H
+  | [ H : In _ _ |- _ ] => inversion H; clear H
+  | [ H : _ /\ _ |- _ ] => invert H
+  | [ H : (_ :: _) = _ |- _ ] => invert H
+  end.
+
+Ltac rw_step :=
+  match goal with
+  | [ H : RealWorld.step_universe _ _ |- _ ] => invert H
+  | [ H : RealWorld.step_user _ _ _ |- _ ] => invert H
+  end.
+
+Ltac doit :=
+  repeat (rw_step; repeat fixcontext).
+
+Hint Constructors Forall.
+Hint Unfold simulates.
+
+Ltac process1 :=
+  match goal with
+  | [ H : simulates _ _ _ |- _ ] => invert H
+  | [ H : exists _, _ |- _ ] => invert H
+  | [ H : _ /\ _ |- _ ] => invert H
+  end.
+
+Ltac process := repeat process1.
+
+  (* Lemma shouldStepOrDone : *)
+  (*   forall {A} {U1 U1' : IdealWorld.universe A} *)
+  (*     {U2 : RealWorld.universe A} *)
+  (*     {R : IdealWorld.universe A -> RealWorld.universe A -> Prop}, *)
+  (*     simulates R U1 U2 *)
+  (*     -> IdealWorld.step_universe^* U1 U1' *)
+  (*     -> idealWorldIsReallyFinalState U1' *)
+  (*     -> idealWorldIsReallyFinalState U1 (* already there! *) *)
+  (*       \/ (exists U1'' U2', IdealWorld.step_universe U1 U1'' *)
+  (*                      /\ IdealWorld.step_universe^* U1'' U1' *)
+  (*                      /\ RealWorld.step_universe^* U2 U2' *)
+  (*                      /\ simulates R U1'' U2'). *)
+  (* Proof. *)
+  (*   intros. *)
+
+  (*   invert H0; process; eauto. *)
+
+  (*   right. *)
+  (*   eapply H0 in H4; eauto; process. eexists. eexists. propositional; eauto. *)
+  (* Qed. *)
+
+Lemma realWorldManyStepsIdealWorldToo :
+  forall {A} {U1 U1': RealWorld.universe A} {R},
+    RealWorld.step_universe^* U1 U1'
+    -> forall U2, simulates R U1 U2
+            -> exists U2', IdealWorld.step_universe^* U2 U2'
+                     /\ simulates R U1' U2'.
+Proof.
+  induct 1; intros; eauto.
+
+  process;
+    (* Step forward *)
+    (match goal with
+     | [ H : (forall _ _, R _ _ -> forall _, _ -> exists _, _) , H1 : R _ _ |- _ ] => eapply H in H1; eauto
+     end); process;
+    (* Apply induction hypothesis *)
+    match goal with
+    | [ H : R ?x ?y , IH : forall _, _ -> _ |- _ ]
+      => assert (S : simulates R x y) by (unfold simulates; propositional); apply IH in S
+    end; process;
+    (* Pick correct final state *)
+    match goal with
+    | [ H : R z ?x |- _ ] => exists x
+    end; propositional; eauto using trc_trans.
+Qed.
+
+Lemma refines_implies_inclusion :
+  forall A (U1 : RealWorld.universe A) (U2 : IdealWorld.universe A),
+    U1 <| U2
+    -> finalAnswerInclusion U1 U2.
+Proof.
+  unfold finalAnswerInclusion, refines in *. intros.
+  process;
+    match goal with
+    | [ H : RealWorld.step_universe ^* _ _ |- _ ] => eapply realWorldManyStepsIdealWorldToo in H
+    end; process; eauto.
+Qed.
