KeyManagement/PingProtocol.v
@@ -1,0 +1,420 @@
+From Coq Require Import List.
+(* Require Import Frap Eqdep. *)
+Require Import Frap.
+
+Require Import Common.
+Require Import Simulation.
+Require IdealWorld.
+Require RealWorld.
+
+Import IdealWorld.IdealNotations.
+Import RealWorld.RealWorldNotations.
+
+Set Implicit Arguments.
+
+Section IdealPing.
+
+  Import IdealWorld.
+
+  Example ideal_ping_universe : universe nat :=
+    {| channel_vector := $0 $+ (0, { })
+     ; users := [
+        (0, {| perms    := $0 $+ (0, {| read := true ; write := true |})
+             ; protocol := (
+                 _ <- (Send (Content 1) 0)
+               ; Return 42)
+            |})
+      ; (1, {| perms    := $0 $+ (0, {| read := true ; write := true |})
+             ; protocol := (
+                 r <- (Recv 0)
+               ; Return match extractContent r with Some c => c | None => 43 end)
+            |})
+               ]
+    |}.
+
+  Check ideal_ping_universe.
+
+End IdealPing.
+
+Section RealPing.
+
+  Import RealWorld.
+
+  Example real_ping : list (user_data nat) :=
+    {| usrid    := 0
+     ; key_heap := $0
+     ; protocol := (  _ <- Send 1 (Plaintext 1)
+                    ; Return 42)
+    |}
+      ::
+    {| usrid    := 1
+     ; key_heap := $0
+     ; protocol := (  rec <- Recv (A := nat)
+                    ; Return (match extractPlainText rec with
+                              | Some msg => msg
+                              | None     => 98
+                              end))
+    |}
+      :: [].
+
+  Example real_ping_universe : universe nat :=
+    {|
+      users            := map (fun u_d => (u_d.(usrid), u_d)) real_ping
+    ; users_msg_buffer := $0
+    ; all_keys         := $0
+    ; all_ciphers      := $0
+    |}.
+
+  Check real_ping_universe.
+
+End RealPing.
+
+(** The correctness theorem for the very simple ping protocol  *)
+Section SimplePingProtocolCorrect.
+
+  Inductive R_ping : RealWorld.universe nat -> IdealWorld.universe nat -> Prop :=
+  | StartPingProtocol :
+      R_ping
+        {|
+          RealWorld.users   := ([
+               (0, {| RealWorld.usrid    := 0
+                    ; RealWorld.key_heap := $0
+                    ; RealWorld.protocol := (
+                        _ <- RealWorld.Send 1 (RealWorld.Plaintext 1)
+                      ; RealWorld.Return 42) |})
+
+             ; (1, {| RealWorld.usrid    := 1
+                    ; RealWorld.key_heap := $0
+                    ; RealWorld.protocol := (
+                        rec <- RealWorld.Recv (A := nat)
+                      ; RealWorld.Return (match RealWorld.extractPlainText rec with
+                                          | Some msg => msg
+                                          | None     => 98
+                                          end)) |})
+                               ])%realworld
+        ; RealWorld.users_msg_buffer := $0
+        ; RealWorld.all_keys         := $0
+        ; RealWorld.all_ciphers      := $0
+        |}
+        {| IdealWorld.channel_vector := $0 $+ (0, {})
+         ; IdealWorld.users := ([
+              (0, {| IdealWorld.perms    := $0 $+ (0, {| IdealWorld.read := true ; IdealWorld.write := true |})
+                   ; IdealWorld.protocol := (
+                        _ <- (IdealWorld.Send (IdealWorld.Content 1) 0)
+                     ; IdealWorld.Return 42)
+                  |})
+            ; (1, {| IdealWorld.perms    := $0 $+ (0, {| IdealWorld.read := true ; IdealWorld.write := true |})
+                   ; IdealWorld.protocol := (
+                       r <- (IdealWorld.Recv 0)
+                     ; IdealWorld.Return match IdealWorld.extractContent r with Some c => c | None => 43 end)
+                  |})
+                               ])%idealworld
+        |}
+
+
+  | SendPing :
+      R_ping
+        {|
+          RealWorld.users   := ([
+               (0, {| RealWorld.usrid    := 0
+                    ; RealWorld.key_heap := $0
+                    ; RealWorld.protocol := _ <- RealWorld.Return tt ; RealWorld.Return 42 |} )
+
+             ; (1, {| RealWorld.usrid    := 1
+                    ; RealWorld.key_heap := $0
+                    ; RealWorld.protocol := (
+                        rec <- RealWorld.Recv (A := nat)
+                      ; RealWorld.Return (match RealWorld.extractPlainText rec with
+                                          | Some msg => msg
+                                          | None     => 98
+                                          end)) |})
+                               ])%realworld
+        ; RealWorld.users_msg_buffer := $0 $+ (1, [RealWorld.Exm (RealWorld.Plaintext 1)])
+        ; RealWorld.all_keys         := $0
+        ; RealWorld.all_ciphers      := $0
+        |}
+        {| IdealWorld.channel_vector := $0 $+ (0, {IdealWorld.Exm (IdealWorld.Content 1)})
+         ; IdealWorld.users := ([
+              (0, {| IdealWorld.perms    := $0 $+ (0, {| IdealWorld.read := true ; IdealWorld.write := true |})
+                   ; IdealWorld.protocol := _ <- IdealWorld.Return tt ; IdealWorld.Return 42
+                  |})
+            ; (1, {| IdealWorld.perms    := $0 $+ (0, {| IdealWorld.read := true ; IdealWorld.write := true |})
+                   ; IdealWorld.protocol := (
+                       r <- (IdealWorld.Recv 0)
+                     ; IdealWorld.Return match IdealWorld.extractContent r with Some c => c | None => 43 end)
+                  |})
+                               ])%idealworld
+        |}
+
+ 
+  | SimplAfterSendPing :
+      R_ping
+        {|
+          RealWorld.users   := ([
+               (0, {| RealWorld.usrid    := 0
+                    ; RealWorld.key_heap := $0
+                    ; RealWorld.protocol := RealWorld.Return 42 |} )
+
+             ; (1, {| RealWorld.usrid    := 1
+                    ; RealWorld.key_heap := $0
+                    ; RealWorld.protocol := (
+                        rec <- RealWorld.Recv (A := nat)
+                      ; RealWorld.Return (match RealWorld.extractPlainText rec with
+                                          | Some msg => msg
+                                          | None     => 98
+                                          end)) |})
+                               ])%realworld
+        ; RealWorld.users_msg_buffer := $0 $+ (1, [RealWorld.Exm (RealWorld.Plaintext 1)])
+        ; RealWorld.all_keys         := $0
+        ; RealWorld.all_ciphers      := $0
+        |}
+        {| IdealWorld.channel_vector := $0 $+ (0, {IdealWorld.Exm (IdealWorld.Content 1)})
+         ; IdealWorld.users := ([
+              (0, {| IdealWorld.perms    := $0 $+ (0, {| IdealWorld.read := true ; IdealWorld.write := true |})
+                   ; IdealWorld.protocol := IdealWorld.Return 42
+                  |})
+            ; (1, {| IdealWorld.perms    := $0 $+ (0, {| IdealWorld.read := true ; IdealWorld.write := true |})
+                   ; IdealWorld.protocol := (
+                       r <- (IdealWorld.Recv 0)
+                     ; IdealWorld.Return match IdealWorld.extractContent r with Some c => c | None => 43 end)
+                  |})
+                               ])%idealworld
+        |}
+
+
+  | ReceivePing :
+      R_ping
+        {|
+          RealWorld.users   := ([
+               (0, {| RealWorld.usrid    := 0
+                    ; RealWorld.key_heap := $0
+                    ; RealWorld.protocol := _ <- RealWorld.Return tt ; RealWorld.Return 42 |} )
+
+             ; (1, {| RealWorld.usrid    := 1
+                    ; RealWorld.key_heap := $0
+                    ; RealWorld.protocol := ( rec <- RealWorld.Return (RealWorld.Plaintext 1)
+                                            ; RealWorld.Return (match RealWorld.extractPlainText rec with
+                                                                | Some msg => msg
+                                                                | None     => 98
+                                                                end)) |})
+                               ])%realworld
+        ; RealWorld.users_msg_buffer := $0
+        ; RealWorld.all_keys         := $0
+        ; RealWorld.all_ciphers      := $0
+        |}
+        {| IdealWorld.channel_vector := $0 $+ (0, {IdealWorld.Exm (IdealWorld.Content 1)})
+         ; IdealWorld.users := ([
+              (0, {| IdealWorld.perms    := $0 $+ (0, {| IdealWorld.read := true ; IdealWorld.write := true |})
+                   ; IdealWorld.protocol := _ <- IdealWorld.Return tt ; IdealWorld.Return 42
+                  |})
+            ; (1, {| IdealWorld.perms    := $0 $+ (0, {| IdealWorld.read := true ; IdealWorld.write := true |})
+                   ; IdealWorld.protocol := ( r <- IdealWorld.Return (IdealWorld.Content 1)
+                                            ; IdealWorld.Return match IdealWorld.extractContent r with Some c => c | None => 43 end)
+                  |})
+                               ])%idealworld
+        |}
+
+
+  | ReceivePingAfterSimplify :
+      R_ping
+        {|
+          RealWorld.users   := ([
+               (0, {| RealWorld.usrid    := 0
+                    ; RealWorld.key_heap := $0
+                    ; RealWorld.protocol := RealWorld.Return 42 |} )
+
+             ; (1, {| RealWorld.usrid    := 1
+                    ; RealWorld.key_heap := $0
+                    ; RealWorld.protocol := ( rec <- RealWorld.Return (RealWorld.Plaintext 1)
+                                            ; RealWorld.Return (match RealWorld.extractPlainText rec with
+                                                                | Some msg => msg
+                                                                | None     => 98
+                                                                end)) |})
+                               ])%realworld
+        ; RealWorld.users_msg_buffer := $0
+        ; RealWorld.all_keys         := $0
+        ; RealWorld.all_ciphers      := $0
+        |}
+        {| IdealWorld.channel_vector := $0 $+ (0, {IdealWorld.Exm (IdealWorld.Content 1)})
+         ; IdealWorld.users := ([
+              (0, {| IdealWorld.perms    := $0 $+ (0, {| IdealWorld.read := true ; IdealWorld.write := true |})
+                   ; IdealWorld.protocol := IdealWorld.Return 42
+                  |})
+            ; (1, {| IdealWorld.perms    := $0 $+ (0, {| IdealWorld.read := true ; IdealWorld.write := true |})
+                   ; IdealWorld.protocol := ( r <- IdealWorld.Return (IdealWorld.Content 1)
+                                            ; IdealWorld.Return match IdealWorld.extractContent r with Some c => c | None => 43 end)
+                  |})
+                               ])%idealworld
+        |}
+
+  | SimplifyBindAfterReceive :
+      R_ping
+        {|
+          RealWorld.users   := ([
+               (0, {| RealWorld.usrid    := 0
+                    ; RealWorld.key_heap := $0
+                    ; RealWorld.protocol := _ <- RealWorld.Return tt ; RealWorld.Return 42 |} )
+
+             ; (1, {| RealWorld.usrid    := 1
+                    ; RealWorld.key_heap := $0
+                    ; RealWorld.protocol := RealWorld.Return 1 |})
+                               ])%realworld
+        ; RealWorld.users_msg_buffer := $0
+        ; RealWorld.all_keys         := $0
+        ; RealWorld.all_ciphers      := $0
+        |}
+        {| IdealWorld.channel_vector := $0 $+ (0, {IdealWorld.Exm (IdealWorld.Content 1)})
+         ; IdealWorld.users := ([
+              (0, {| IdealWorld.perms    := $0 $+ (0, {| IdealWorld.read := true ; IdealWorld.write := true |})
+                   ; IdealWorld.protocol := _ <- IdealWorld.Return tt ; IdealWorld.Return 42
+                  |})
+            ; (1, {| IdealWorld.perms    := $0 $+ (0, {| IdealWorld.read := true ; IdealWorld.write := true |})
+                   ; IdealWorld.protocol := IdealWorld.Return 1
+                  |})
+                               ])%idealworld
+        |}
+
+
+  | Finish :
+      R_ping
+        {|
+          RealWorld.users   := ([
+               (0, {| RealWorld.usrid    := 0
+                    ; RealWorld.key_heap := $0
+                    ; RealWorld.protocol := RealWorld.Return 42 |} )
+
+             ; (1, {| RealWorld.usrid    := 1
+                    ; RealWorld.key_heap := $0
+                    ; RealWorld.protocol := RealWorld.Return 1 |} )
+                               ])%realworld
+        ; RealWorld.users_msg_buffer := $0
+        ; RealWorld.all_keys         := $0
+        ; RealWorld.all_ciphers      := $0
+        |}
+        {| IdealWorld.channel_vector := $0 $+ (0, {IdealWorld.Exm (IdealWorld.Content 1)})
+         ; IdealWorld.users := ([
+              (0, {| IdealWorld.perms    := $0 $+ (0, {| IdealWorld.read := true ; IdealWorld.write := true |})
+                   ; IdealWorld.protocol := IdealWorld.Return 42
+                  |})
+            ; (1, {| IdealWorld.perms    := $0 $+ (0, {| IdealWorld.read := true ; IdealWorld.write := true |})
+                   ; IdealWorld.protocol := IdealWorld.Return 1
+                  |})
+                               ])%idealworld
+        |}
+  .
+
+  Hint Constructors R_ping.
+  Hint Resolve in_eq in_cons.
+
+  Lemma finalStatesAre : 
+    forall {U1 : RealWorld.universe nat} {U2 : IdealWorld.universe nat},
+      R_ping U1 U2
+      -> realWorldIsReallyFinalState U1
+      -> U1 = {|
+          RealWorld.users :=
+            [(0, {| RealWorld.usrid := 0; RealWorld.key_heap := $0; RealWorld.protocol := RealWorld.Return 42 |});
+             (1, {| RealWorld.usrid := 1; RealWorld.key_heap := $0; RealWorld.protocol := RealWorld.Return  1 |})];
+          RealWorld.users_msg_buffer := $0;
+          RealWorld.all_keys := $0;
+          RealWorld.all_ciphers := $0 |}
+        /\ U2 = {|
+            IdealWorld.channel_vector := $0 $+ (0, {IdealWorld.Exm (IdealWorld.Content 1)});
+            IdealWorld.users :=
+              [(0, {|
+                  IdealWorld.protocol := IdealWorld.Return 42;
+                  IdealWorld.perms := $0 $+ (0, {| IdealWorld.read := true; IdealWorld.write := true |}) |});
+                 (1, {|
+                    IdealWorld.protocol := IdealWorld.Return 1;
+                    IdealWorld.perms := $0 $+ (0, {| IdealWorld.read := true; IdealWorld.write := true |}) |})]
+          |}.
+  Proof.
+    intros.
+
+    destruct H;
+      (repeat match goal with
+              | [ H : realWorldIsReallyFinalState _ |- _ ] => invert H
+              | [ H : exists a , _ = RealWorld.Return a |- _ ] => invert H
+              | [ H : _ = RealWorld.Return _ |- _ ] => invert H
+              | [ H : Forall _ _ |- _ ] => invert H
+              end); propositional.
+  Qed.
+
+  Hint Resolve finalStatesAre.
+
+  Lemma rping_steps_simulate : 
+    forall U1 U2,
+      R_ping U1 U2
+      -> forall U1',
+        RealWorld.step_universe U1 U1'
+        -> exists U2',
+          IdealWorld.step_universe^* U2 U2'
+          /\ R_ping U1' U2'.
+  Proof.
+
+    Hint Extern 1 (In _ (IdealWorld.users _)) => progress simpl.
+    Hint Extern 1 (_ \in _ ) => sets.
+    Hint Extern 1 (IdealWorld.step_user (_, IdealWorld.Bind _ _, _) _) => eapply IdealWorld.StepBindRecur; simplify.
+    Hint Extern 1 (IdealWorld.step_user (_, IdealWorld.Send _ _, _) _) => eapply IdealWorld.StepSend'; simplify.
+    Hint Extern 1 (IdealWorld.step_user (IdealWorld.channel_vector _, _, _) _) => progress simpl.
+
+    Hint Extern 1 (R_ping (RealWorld.updateUniverse _ _ _ _ _ _ _) _ ) =>
+      autorewrite with core; unfold RealWorld.updateUniverse, RealWorld.multiMapAdd; simplify.
+    (* Hint Extern 1 (R_ping (RealWorld.updateUniverse _ _ _ _ _ _ _) _ ) => *)
+    (*   unfold RealWorld.updateUniverse, RealWorld.multiMapAdd; autorewrite with core; simplify. *)
+
+    intros.
+
+    (* The main idea for solving the generated (existential) goals here is to split apart the
+     * conjunction and then solve the second one first.  This works because the second conjuct is
+     * the simulation relation constructor, which helps lock down the destsination state and helps
+     * determine how many steps are needed to get there in the ideal world. Otherwise, we seem to just
+     * pick "take no steps" and get stuck.  *)
+    Hint Extern 1 (exists _, _ /\ _) => eexists; constructor; simplify; [ | constructor ].
+
+    invert H; doit; simpl in *; eauto 8;
+      (* Question for Adam.  This works, but pulling the rewrite out breaks it.
+         despite the fact that the Extern above with the needed rewrite is
+         firing.  *)
+      autorewrite with core;
+      eauto 12.
+  Qed.
+
+  Lemma rping_finishes_correctly :
+    forall U1 U2,
+      R_ping U1 U2
+      -> realWorldIsReallyFinalState U1
+      -> idealWorldIsReallyFinalState U2
+        /\ realWorldReturnsOf U1 = idealWorldReturnsOf U2.
+  Proof.
+    Hint Extern 1 (exists _, _ = _) => eexists; simplify; reflexivity.
+    Hint Extern 1 (idealWorldIsReallyFinalState _) => unfold idealWorldIsReallyFinalState; simplify.
+    Hint Constructors Forall.
+
+    firstorder;
+      (match goal with
+       | [ H : R_ping _ _ |- _ ] => apply finalStatesAre in H
+       end); repeat fixcontext; simplify; eauto 8.
+
+  Qed.
+
+  Hint Resolve rping_steps_simulate rping_finishes_correctly.
+
+  Theorem idealPingRefinesRealPing : 
+    real_ping_universe <| ideal_ping_universe.
+  Proof.
+    exists R_ping.
+    assert (F := rping_finishes_correctly).
+    unfold simulates; firstorder; eauto.
+
+    (* invert H; doit; simpl in *; try contradiction; eexists; *)
+    (*   (constructor; [ | simplify; constructor ]; eauto 8; eauto 10). *)
+  Qed.
+
+  Theorem ping_protocol_ok :
+    finalAnswerInclusion real_ping_universe ideal_ping_universe.
+  Proof.
+    apply refines_implies_inclusion.
+    apply idealPingRefinesRealPing.
+  Qed.
+
+End SimplePingProtocolCorrect.
